feat: prove that regular languages are closed under Kleene star (#241)
This patch proves that regular languages are closed under Kleene star.
The proof technique is similar to the one used in PR
https://github.com/leanprover/cslib/pull/239 and re-uses much of the
infrastructure introduce in that PR.

---------

Co-authored-by: Chris Henson <chrishenson.net@gmail.com>

Cslib/Computability/Automata/NA/Loop.lean
@@ -6,7 +6,7 @@ Authors: Ching-Tsun Chou
 
 module
 
-public import Cslib.Computability.Automata.NA.Basic
+public import Cslib.Computability.Automata.NA.Total
 public import Cslib.Foundations.Data.OmegaSequence.Temporal
 
 @[expose] public section
@@ -15,7 +15,7 @@ public import Cslib.Foundations.Data.OmegaSequence.Temporal
 
 namespace Cslib.Automata.NA
 
-open Nat List Sum ωSequence Acceptor Language
+open Nat Set Sum ωSequence Acceptor Language
 open scoped Run LTS
 
 variable {Symbol State : Type*}
@@ -81,23 +81,24 @@ lemma loop_run_from_left {xs : ωSequence Symbol} {ss : ωSequence (Unit ⊕ Sta
 
 /-- A run of `na.loop` containing at least one non-initial `()` state is the concatenation
 of a nonempty finite run of `na` followed by a run of `na.loop`. -/
-theorem loop_run_one_iter {xs : ωSequence Symbol} {ss : ωSequence (Unit ⊕ State)}
-    (h : na.loop.Run xs ss) (h1 : ∃ k, 0 < k ∧ (ss k).isLeft) :
-    ∃ n, xs.take n ∈ language na - 1 ∧ na.loop.Run (xs.drop n) (ss.drop n) := by
-  let n := Nat.find h1
-  have : 0 < n ∧ (ss n).isLeft := Nat.find_spec h1
-  have : ∀ k, 0 < k → k < n → (ss k).isRight := by grind [Nat.find_min h1]
-  refine ⟨n, ⟨?_, ?_⟩, ?_⟩
+theorem loop_run_one_iter {xs : ωSequence Symbol} {ss : ωSequence (Unit ⊕ State)} {k : ℕ}
+    (h : na.loop.Run xs ss) (h1 : 0 < k) (h2 : (ss k).isLeft) :
+    ∃ n, n ≤ k ∧ xs.take n ∈ language na - 1 ∧ na.loop.Run (xs.drop n) (ss.drop n) := by
+  have h1' : ∃ k, 0 < k ∧ (ss k).isLeft := by grind
+  let n := Nat.find h1'
+  have : 0 < n ∧ (ss n).isLeft := Nat.find_spec h1'
+  have : ∀ k, 0 < k → k < n → (ss k).isRight := by grind [Nat.find_min h1']
+  refine ⟨n, by grind, ⟨?_, ?_⟩, ?_⟩
   · grind [loop_run_left_right_left]
   · have neq : (ωSequence.take n xs).length ≠ 0 := by grind
-    exact neq.imp (congrArg length)
+    exact neq.imp (congrArg List.length)
   · grind [loop_run_from_left]
 
 /-- For any finite word in `language na`, there is a corresponding finite run of `na.loop`. -/
 theorem loop_fin_run_exists {xl : List Symbol} (h : xl ∈ language na) :
     ∃ sl : List (Unit ⊕ State), ∃ _ : sl.length = xl.length + 1,
     sl[0] = inl () ∧ sl[xl.length] = inl () ∧
-    ∀ k, ∀ _ : k < xl.length, na.loop.Tr sl[k] xl[k] sl[k + 1] := by
+    ∀ k, (_ : k < xl.length) → na.loop.Tr sl[k] xl[k] sl[k + 1] := by
   obtain ⟨_, _, _, _, h_mtr⟩ := h
   obtain ⟨sl, _, _, _, _⟩ := LTS.MTr.exists_states h_mtr
   by_cases xl.length = 0
@@ -105,6 +106,15 @@ theorem loop_fin_run_exists {xl : List Symbol} (h : xl ∈ language na) :
     grind
   · use [inl ()] ++ (sl.extract 1 xl.length).map inr ++ [inl ()]
     grind [FinAcc.loop]
+
+/-- For any finite word in `language na`, there is a corresponding multistep transition
+of `na.loop`. -/
+theorem loop_fin_run_mtr {xl : List Symbol} (h : xl ∈ language na) :
+    na.loop.MTr (inl ()) xl (inl ()) := by
+  obtain ⟨sl, _, _, _, h_run⟩ := loop_fin_run_exists h
+  suffices ∀ k, (_ : k ≤ xl.length) → na.loop.MTr (inl ()) (xl.take k) sl[k] by grind
+  intro k
+  induction k <;> grind [LTS.MTr.stepR, List.take_add_one]
 
 /-- For any infinite sequence `xls` of nonempty finite words from `language na`,
 there is an infinite run of `na.loop` corresponding to `xls.flatten` in which
@@ -118,7 +128,7 @@ theorem loop_run_exists [Inhabited Symbol] {xls : ωSequence (List Symbol)}
   choose sls h_sls using fun k ↦ loop_fin_run_exists <| (h k).left
   let segs := ωSequence.mk fun k ↦ (sls k).take (xls k).length
   have h_len : xls.cumLen = segs.cumLen := by ext k; induction k <;> grind
-  have h_pos (k : ℕ) : (segs k).length > 0 := by grind [eq_nil_iff_length_eq_zero]
+  have h_pos (k : ℕ) : (segs k).length > 0 := by grind [List.eq_nil_iff_length_eq_zero]
   have h_mono := cumLen_strictMono h_pos
   have h_zero := cumLen_zero (ls := segs)
   have h_seg0 (k : ℕ) : (segs k)[0]! = inl () := by grind
@@ -148,8 +158,9 @@ theorem loop_language_eq [Inhabited Symbol] :
   apply le_antisymm
   · apply omegaPow_coind
     rintro xs ⟨ss, h_run, h_acc⟩
-    have h1 : ∃ k > 0, (ss k).isLeft := by grind [FinAcc.loop, frequently_atTop'.mp h_acc 0]
-    obtain ⟨n, _⟩ := loop_run_one_iter h_run h1
+    obtain ⟨k, h1, h2⟩ : ∃ k > 0, (ss k).isLeft :=
+      by grind [FinAcc.loop, frequently_atTop'.mp h_acc 0]
+    obtain ⟨n, _⟩ := loop_run_one_iter h_run h1 h2
     refine ⟨xs.take n, by grind, xs.drop n, ?_, by simp⟩
     refine ⟨ss.drop n, by grind, ?_⟩
     apply (drop_frequently_iff_frequently n).mpr
@@ -160,8 +171,62 @@ theorem loop_language_eq [Inhabited Symbol] :
     use ss, h_run
     apply frequently_iff_strictMono.mpr
     use xls.cumLen, ?_, by grind
-    grind [cumLen_strictMono, eq_nil_iff_length_eq_zero]
+    grind [cumLen_strictMono, List.eq_nil_iff_length_eq_zero]
 
 end Buchi
+
+namespace FinAcc
+
+open scoped Computability
+
+/-- `finLoop na` is the loop construction applied to the "totalized" version of `na`. -/
+def finLoop (na : FinAcc State Symbol) : NA (Unit ⊕ (State ⊕ Unit)) Symbol :=
+  FinAcc.loop ⟨na.totalize, inl '' na.accept⟩
+
+/-- `finLoop na` is total, assuming that `na` has at least one start state. -/
+instance [h : Nonempty na.start] : na.finLoop.Total where
+  total s x := match s with
+    | inl _ => ⟨inr (inr ()), by simpa [finLoop, loop, NA.totalize, LTS.totalize] using h⟩
+    | inr _ => ⟨inr (inr ()), by grind [finLoop, loop, NA.totalize, LTS.totalize]⟩
+
+/-- `finLoop na` accepts the Kleene star of the language of `na`, assuming that
+the latter is nonempty. -/
+theorem loop_language_eq [Inhabited Symbol] (h : ¬ language na = 0) :
+    language (FinAcc.mk na.finLoop {inl ()}) = (language na)∗ := by
+  rw [Language.kstar_iff_mul_add]
+  ext xl; constructor
+  · rintro ⟨s, _, t, h_acc, h_mtr⟩
+    by_cases h_xl : xl = []
+    · grind [mem_add, mem_one]
+    · have : Nonempty na.start := by
+        obtain ⟨_, s0, _, _⟩ := nonempty_iff_ne_empty.mpr h
+        use s0
+      obtain ⟨xs, ss, h_ωtr, rfl, rfl⟩ := LTS.Total.mTr_ωTr h_mtr
+      have h_run : na.finLoop.Run (xl ++ω xs) ss := by grind [Run]
+      obtain ⟨h1, h2⟩ : 0 < xl.length ∧ (ss xl.length).isLeft := by
+        simp only [mem_singleton_iff] at h_acc
+        grind
+      obtain ⟨n, h_n, _, _, h_ωtr'⟩ := loop_run_one_iter h_run h1 h2
+      left; refine ⟨xl.take n, ?_, xl.drop n, ?_, ?_⟩
+      · grind [totalize_language_eq, take_append_of_le_length]
+      · refine ⟨ss n, by grind, ss xl.length, by grind, ?_⟩
+        have := LTS.ωTr_mTr h_ωtr' (show 0 ≤ xl.length - n by grind)
+        have : n + (xl.length - n) = xl.length := by grind
+        have : ((xl ++ω xs).drop n).extract 0 (xl.length - n) = xl.drop n := by
+          grind [extract_eq_take, drop_append_of_le_length, take_append_of_le_length]
+        grind [finLoop]
+      · exact xl.take_append_drop n
+  · rintro (h | h)
+    · obtain ⟨xl1, ⟨h_xl1, _⟩, xl2, h_xl2, rfl⟩ := h
+      rw [← totalize_language_eq] at h_xl1
+      have := loop_fin_run_mtr h_xl1
+      obtain ⟨s1, _, s2, _, _⟩ := h_xl2
+      obtain ⟨rfl⟩ : s1 = inl () := by grind [finLoop, loop]
+      obtain ⟨rfl⟩ : s2 = inl () := by grind [finLoop, loop]
+      refine ⟨inl (), ?_, inl (), ?_, LTS.MTr.comp _ this ?_⟩ <;> assumption
+    · obtain ⟨rfl⟩ := (Language.mem_one xl).mp h
+      refine ⟨inl (), ?_, inl (), ?_, ?_⟩ <;> grind [finLoop, loop]
+
+end FinAcc
 
 end Cslib.Automata.NA
